proof/X-Wing-Correction-Proof.ec
@@ -1,0 +1,23 @@
+require import AllCore IntDiv CoreMap List Distr.
+
+from Jasmin require import JModel_x86.
+
+import SLH64.
+require import XWing_Spec XWing_Helper_Functions CorrectnessProof_Mulx Mulx_scalarmult_s Jkem_avx2_stack FIPS202_SHA3 MLKEM.
+require import Array4 Array6 Array8 Array32 Array64 Array96 Array140 Array152 Array1088 Array1120 Array1184 Array1216 Array2400.
+require import WArray4 WArray6 WArray32 WArray64 WArray96 WArray1088 WArray1120 WArray1184 WArray1216 WArray2400.
+
+
+op SHA3_256_A128_A6 : W8.t Array32.t -> W8.t Array32.t -> W8.t Array32.t -> W8.t Array32.t -> W8.t Array32.t -> W8.t Array32.t.
+op SHAKE256_A96_A32 : W8.t Array96.t -> W8.t Array32.t -> W8.t Array96.t.
+
+
+axiom sha3_256_A128__A6 ss ss_mlkem ss_x25519 ct_25519 pk_25519 :
+   phoare [M._sha3_256_A128__A6 :
+               arg = (ss, ss_mlkem, ss_x25519, ct_25519, pk_25519) ==>
+               res = SHA3_256_A128_A6 ss ss_mlkem ss_x25519 ct_25519 pk_25519] = 1%r.
+
+axiom shake256_A96_A32 out inp :
+   phoare [M._shake256_A96__A32 :
+               arg = (out, inp) ==>
+               res = SHAKE256_A96_A32 out inp] = 1%r.
